{
  "@context": {
    "rdf": "https://www.w3.org/1999/02/22-rdf-syntax-ns#",
    "rdfs": "https://www.w3.org/2000/01/rdf-schema#",
    "schema": "https://schema.org/",
    "webiot": "https://schema.iot.webizing.org/",
    "xsd": "https://www.w3.org/2001/XMLSchema#"
  },
  "@graph": [
    {
      "@id": "webiot:EnergyApplianceMonitor",
      "@type": "rdfs:Class",
      "rdfs:comment": "EnergyApplianceMonitor Sensor - 공기질 로깅 ex)Foobot(5분 주기로 데이터를 가져옴)",
      "rdfs:label": "EnergyApplianceMonitor",
      "schema:sameAs": {
        "@id": "webiot:EnergyApplianceMonitor"
      }
    },
    {
      "@id": "webiot:applianceId",
      "@type": "rdf:Property",
      "rdfs:comment": "가전제품 Id",
      "rdfs:label": "applianceId",
      "schema:rangeIncludes": {
        "@id": "schema:Text"
      }
    },
    {
      "@id": "webiot:location",
      "@type": "rdf:Property",
      "rdfs:comment": "location of the sensor - format: free",
      "rdfs:label": "location",
      "schema:rangeIncludes": {
        "@id": "schema:Text"
      }
    },
    {
      "@id": "webiot:activePower",
      "@type": "rdf:Property",
      "rdfs:comment": "appliance activePower - unit: W, 양수: On, 음수: Off",
      "rdfs:label": "activePower",
      "schema:rangeIncludes": {
        "@id": "schema:Float"
      }
    },
    {
      "@id": "webiot:address",
      "@type": "rdf:Property",
      "rdfs:comment": "building where the sensor resides - format: organization-building ex)yongjaelee-house, kist-l1, kist-l8",
      "rdfs:label": "address",
      "schema:rangeIncludes": {
        "@id": "schema:Text"
      }
    },
    {
      "@id": "webiot:room",
      "@type": "rdf:Property",
      "rdfs:comment": "room number of the building where the sensor resides - ex) L8321",
      "rdfs:label": "room",
      "schema:rangeIncludes": {
        "@id": "schema:Text"
      }
    },
    {
      "@id": "webiot:user",
      "@type": "rdf:Property",
      "rdfs:comment": "user of the sensor - format: firstName+LastName ex)jonghoLee, wanhoIm",
      "rdfs:label": "user",
      "schema:rangeIncludes": {
        "@id": "schema:Text"
      }
    },
    {
      "@id": "webiot:time",
      "@type": "rdf:Property",
      "rdfs:comment": "time at which the data measurement was made - ex)2017-05-30T18:54:20+09:00",
      "rdfs:label": "time",
      "schema:rangeIncludes": {
        "@id": "schema:DateTime"
      }
    },
    {
      "@id": "webiot:name",
      "@type": "rdf:Property",
      "rdfs:comment": "name of the sensor - format: SensorXX ex)Foobot00, Beddit02",
      "rdfs:label": "name",
      "schema:rangeIncludes": {
        "@id": "schema:Text"
      }
    }
  ]
}
